WIP

code/ecdsa/Hacl.Impl.EC.ScalarMultiplication.WNAF.fst
@@ -26,8 +26,10 @@ open Hacl.Impl.EC.Masking
 open Hacl.Impl.EC.Masking.ScalarAccess
 open Lib.IntTypes.Intrinsics
 
+open FStar.Math.Lemmas
 
-#set-options "--z3rlimit 200" 
+
+#set-options "--z3rlimit 100 --max_fuel 0 --max_ifuel 0" 
 (*  https://www.usenix.org/system/files/conference/usenixsecurity18/sec18-alam.pdf*)
 
 
@@ -35,75 +37,405 @@ inline_for_extraction noextract
 let radix: (r: uint64 {v r == w}) = (u64 5)
 
 inline_for_extraction noextract
-let dradix : (r: uint64 {v r == m}) = (u64 32)
+let radix_shiftval: (r: shiftval U64 {v r == w /\ v r == v radix}) = (size 5)
 
 inline_for_extraction noextract
-let dradix_wnaf : (r: uint64 {v r == 2 * m}) = (u64 64)
+let radix_u32: (r: size_t {v r == w /\ v r == v radix}) = (size 5)
+
+inline_for_extraction noextract
+let dradix : (r: uint64 {v r == m}) = assert_norm(pow2 5 == 32); (u64 32)
+
+inline_for_extraction noextract
+let dradix_wnaf : (r: uint64 {v r == 2 * m}) = 
+  FStar.Math.Lemmas.pow2_double_sum 5; 
+  assert_norm (pow2 6 == 64);
+  (u64 64)
 
 
-val scalar_rwnaf_step_compute_di: w: uint64 -> out: lbuffer uint64 (size ((getPower P256 / Spec.ECC.WNAF.w + 1) * 2))
+val scalar_rwnaf_step_compute_di: #c: curve -> w: uint64 -> out: lbuffer uint64 (size ((getPower c / Spec.ECC.WNAF.w + 1) * 2))
   -> mask: uint64 {v mask = pow2 (v radix + 1) - 1} 
-  -> r: lbuffer uint64 (size 1) -> i: size_t {v i < getPower P256 / Spec.ECC.WNAF.w + 1} -> 
+  -> r: lbuffer uint64 (size 1) -> i: size_t {v i < getPower c / Spec.ECC.WNAF.w + 1} -> 
   Stack unit
   (requires fun h -> live h out /\ live h r)
-  (ensures fun h0 _ h1 -> 
+  (ensures fun h0 _ h1 -> modifies (loc out |+| loc r) h0 h1 /\ (
     let sign = Lib.Sequence.index (as_seq h1 out) (2 * v i + 1) in 
     let abs =  Lib.Sequence.index (as_seq h1 out) (2 * v i) in 
-    if v sign = 0 then v abs = v w - v dradix else v abs = - (v w - v dradix))
+    if v sign = 0 then v w - v dradix == v abs else - (v w - v dradix) == v abs))
 
-let scalar_rwnaf_step_compute_di wVar out mask r i = 
-  let w = logand wVar mask in 
-    logand_mask wVar mask (v radix + 1);
-    FStar.Math.Lemmas.pow2_double_mult (v radix);
-    assert(v w == v wVar % (2 * pow2 (v radix)));
-   
+let scalar_rwnaf_step_compute_di w out mask r i =
+  let h0 = ST.get() in 
   let c = Lib.IntTypes.Intrinsics.sub_borrow_u64 (u64 0) w dradix r in 
   let r0 = index r (size 0) in 
     let h1 = ST.get() in 
-    
-  assert (v r0 - v c * pow2 64 == v w - v dradix);
-  
+
   let r2 = u64 0 -. r0 in 
-    assert(v r2 == (- v r0) % pow2 64);
     
   let cAsFlag = eq1_u64 c in 
   let r3 = cmovznz2 r2 r0 cAsFlag in 
 
   upd out (size 2 *! i) r3;
+  upd out (size 2 *! i +! size 1) cAsFlag
 
+(*
+val shift_left_bit: a: uint64 {v a <= 1} -> i: shiftval U64 {v i < 63} -> 
+  Stack uint64 
+  (requires fun h -> True)
+  (ensures fun h0 r h1 -> v r <= pow2 (v i))
+
+let shift_left_bit a i = shift_left a i 
+*)
+
+val scalar_compute_window_lemma: #c: curve ->  scalar: scalar_bytes #c
+  -> i: size_t {v i < getPower c / Spec.ECC.WNAF.w - 1} ->
+  Lemma (
+    let t = (v i + 1) * w  in 
+    let sh0 = v (ith_bit scalar (t + 1)) in 
+    let sh1 = v (ith_bit scalar (t + 2)) in 
+    let sh2 = v (ith_bit scalar (t + 3)) in 
+    let sh3 = v (ith_bit scalar (t + 4)) in 
+    let sh4 = v (ith_bit scalar (t + 5)) in 
+
+    let i = sh0 * pow2 1 + 
+      sh1 * pow2 2 +
+      sh2 * pow2 3 +
+      sh3 * pow2 4 +
+      sh4 * pow2 5 in 
+  scalar_as_nat_ scalar (v (getScalarLen c) - (t + 1)) % m * 2 == i /\
+  scalar_as_nat scalar / pow2 (t + 1) % m * 2 == i)
+
+
+
+#push-options "--z3rlimit 300"
+
+
+let scalar_compute_window_lemma #c scalar k = 
+  let t = (v k + 1) * w  in 
+  let sh0 = v (ith_bit scalar (t + 1)) in 
+  let sh1 = v (ith_bit scalar (t + 2)) in 
+  let sh2 = v (ith_bit scalar (t + 3)) in 
+  let sh3 = v (ith_bit scalar (t + 4)) in 
+  let sh4 = v (ith_bit scalar (t + 5)) in 
+
+  let i = sh0 * pow2 1 + 
+    sh1 * pow2 2 +
+    sh2 * pow2 3 +
+    sh3 * pow2 4 +
+    sh4 * pow2 5 in 
+    
+  scalar_as_nat_def #c  scalar (v (getScalarLen c) - (t + 1));
+  scalar_as_nat_def #c  scalar (v (getScalarLen c) - (t + 2));
+  scalar_as_nat_def #c  scalar (v (getScalarLen c) - (t + 3));
+  scalar_as_nat_def #c  scalar (v (getScalarLen c) - (t + 4));
+  scalar_as_nat_def #c  scalar (v (getScalarLen c) - (t + 5));
+
+  assume (pow2 2 * 2 == pow2 3);
+  assume (pow2 3 * 2 == pow2 4);
+  assume (pow2 4 * 2 == pow2 5);
+  assume (pow2 5 * 2 == pow2 6);
+
+  assert(2 * scalar_as_nat_ scalar (v (getScalarLen c) - (t + 1)) == 
+    pow2 6 * scalar_as_nat_ scalar (v (getScalarLen c) - (t + 6)) + i);
+
+  assert(2 * scalar_as_nat_ scalar (v (getScalarLen c) - (t + 1)) % pow2 6 == 
+    (pow2 6 * scalar_as_nat_ scalar (v (getScalarLen c) - (t + 6)) + i) % pow2 6); 
+
+  pow2_multiplication_modulo_lemma_2 (scalar_as_nat_ scalar (v (getScalarLen c) - (t + 1))) 6 1;
+
+  assert(scalar_as_nat_ scalar (v (getScalarLen c) - (t + 1)) * 2 % pow2 6 == 
+    (pow2 6 * scalar_as_nat_ scalar (v (getScalarLen c) - (t + 6)) + i) % pow2 6);
+
+  lemma_mod_plus i (scalar_as_nat_ scalar (v (getScalarLen c) - (t + 6))) (pow2 6);
+
+
+  assert(scalar_as_nat_ scalar (v (getScalarLen c) - (t + 1)) % pow2 5 * 2 ==  i % pow2 6);
+
+
+  assume (i < pow2 6);
+  small_mod i (pow2 6);
+
+  Hacl.Impl.EC.Masking.ScalarAccess.Lemmas.test #c scalar ((v (getScalarLen c) - (t + 1)));
+  assert(scalar_as_nat_ scalar (v (getScalarLen c) - (t + 1)) % pow2 5 * 2 == i);
   
-  assert(v r3 == abs (v w - v dradix));
-  assert(if v w < v dradix then v cAsFlag == pow2 64 - 1 else v cAsFlag == 0);
-  assert(if v cAsFlag = 0 then v w - v dradix == v r3 else v w - v dradix == - v r3);
+  assert(scalar_as_nat_ scalar (v (getScalarLen c) - (t + 1)) == scalar_as_nat scalar / pow2 (t + 1));
+  assert(scalar_as_nat scalar / pow2 (t + 1) % m * 2 == i)
 
 
-  upd out (size 2 *! i +! size 1) cAsFlag;
-  admit()
+val scalar_rwnaf_step_compute_window_: #c: curve 
+  -> wStart: uint64 {v wStart < pow2 (64 - 5)}
+  -> scalar: scalar_t #MUT #c 
+  -> k: size_t {v k < getPower c / Spec.ECC.WNAF.w - 1} -> 
+  Stack uint64 
+  (requires fun h -> live h scalar)
+  (ensures fun h0 w0 h1 -> modifies0 h0 h1 /\ v w0 - v wStart = 
+    v (ith_bit (as_seq h0 scalar) ((v k + 1) * w + 1)) * pow2 1 + 
+    v (ith_bit (as_seq h0 scalar) ((v k + 1) * w + 2)) * pow2 2 +
+    v (ith_bit (as_seq h0 scalar) ((v k + 1) * w + 3)) * pow2 3 +
+    v (ith_bit (as_seq h0 scalar) ((v k + 1) * w + 4)) * pow2 4 +
+    v (ith_bit (as_seq h0 scalar) ((v k + 1) * w + 5)) * pow2 5)
 
-
-
-val scalar_rwnaf_step: out: lbuffer uint64 (size 104) -> scalar: lbuffer uint8 (size 32) 
-  -> window: lbuffer uint64 (size 1) -> mask: uint64 -> r: lbuffer uint64 (size 1) -> i: size_t ->  Stack unit 
-  (requires fun h -> True) (ensures fun h0 _ h1 -> True)
-
-let scalar_rwnaf_step out scalar window mask r i = 
+let scalar_rwnaf_step_compute_window_ #c wStart scalar k = 
   let h0 = ST.get() in 
-  let wVar = to_u64 (index window (size 0)) in 
-    assert(v wVar == Lib.Sequence.index (as_seq h0 window) 0);
-  let w = logand wVar mask in 
-
-  scalar_rwnaf_step_compute_di wVar out mask r i; 
+    assert_norm (pow2 (64 - 5) + pow2 1 + pow2 2 + pow2 3 + pow2 4 + pow2 5 < pow2 64);
   
-  let d = w -! dradix in 
-  let wStart = shift_right (wVar -! d) radix in 
+  let i = (size 1 +! k) *! radix_u32 in 
+  let w0 = wStart +! (shift_left (getScalarBit_leftEndian #c scalar (i +! size 1)) (size 1)) in 
+  let w0 = w0 +! (shift_left (getScalarBit_leftEndian #c scalar (i +! (size 2))) (size 2)) in 
+  let w0 = w0 +! (shift_left (getScalarBit_leftEndian #c scalar (i +! (size 3))) (size 3)) in 
+  let w0 = w0 +! (shift_left (getScalarBit_leftEndian #c scalar (i +! (size 4))) (size 4)) in 
+  let w0 = w0 +! (shift_left (getScalarBit_leftEndian #c scalar (i +! (size 5))) (size 5)) in 
 
-  let w0 = wStart +! (shift_left (getScalarBit_leftEndian #P256 scalar ((size 1 +! i) *! radix +! (size 1))) (size 1)) in 
-  let w0 = w0 +! (shift_left (getScalarBit_leftEndian #P256  scalar ((size 1 +! i) *! radix +! (size 2))) (size 2)) in 
-  let w0 = w0 +! (shift_left (getScalarBit_leftEndian #P256  scalar ((size 1 +! i) *! radix +! (size 3))) (size 3)) in 
-  let w0 = w0 +! (shift_left (getScalarBit_leftEndian #P256 scalar ((size 1 +! i) *! radix +! (size 4))) (size 4)) in 
-  let w0 = w0 +! (shift_left (getScalarBit_leftEndian #P256 scalar ((size 1 +! i) *! radix +! (size 5))) (size 5)) in
+  w0
 
-  upd window (size 0) w0
+
+#pop-options
+
+
+val scalar_rwnaf_step_compute_window: #c: curve 
+  -> wStart: uint64 {v wStart < pow2 (64 - 5)}
+  -> scalar: scalar_t #MUT #c 
+  -> k: size_t {v k < getPower c / Spec.ECC.WNAF.w - 1} -> 
+  Stack uint64 
+  (requires fun h -> live h scalar)
+  (ensures fun h0 w0 h1 -> modifies0 h0 h1 /\ (
+    let t = (v k + 1) * w in 
+    scalar_as_nat_ (as_seq h0 scalar) (v (getScalarLen c) - (t + 1)) % m * 2 == v w0 - v wStart /\
+    scalar_as_nat (as_seq h0 scalar) / pow2 (t + 1) % m * 2 == v w0 - v wStart))
+
+let scalar_rwnaf_step_compute_window #c wStart scalar k = 
+  let h0 = ST.get() in 
+  scalar_compute_window_lemma (as_seq h0 scalar) k;
+  scalar_rwnaf_step_compute_window_ #c wStart scalar k  
+
+
+val scalar_rwnaf_step: #c: curve -> out: lbuffer uint64 (size ((getPower c / Spec.ECC.WNAF.w + 1) * 2))
+  -> scalar: scalar_t #MUT #c 
+  -> window: lbuffer uint64 (size 1) 
+  -> mask: uint64 {v mask = pow2 (v radix + 1) - 1}
+  -> r: lbuffer uint64 (size 1) 
+  -> i: size_t {v i < getPower c / Spec.ECC.WNAF.w - 1} ->  Stack unit 
+  (requires fun h -> live h out /\ live h scalar /\ live h window /\ live h r /\ 
+    LowStar.Monotonic.Buffer.all_disjoint [loc out; loc scalar; loc window; loc r] /\ (
+    let w0 = v (Lib.Sequence.index (as_seq h window) 0) in 
+    w0 == scalar_as_nat (as_seq h scalar) % pow2 (v i * w + w + 1) / pow2 (v i * w) / 2 * 2 + 1 /\
+    w0 < 2 * m))
+  (ensures fun h0 _ h1 -> modifies (loc out |+| loc window |+| loc r) h0 h1 /\ (
+    let k = v i + 1 in 
+    let w0 = v (Lib.Sequence.index (as_seq h0 window) 0) in
+    let wUpd = v (Lib.Sequence.index (as_seq h1 window) 0) in
+    let sign = Lib.Sequence.index (as_seq h1 out) (2 * v i + 1) in 
+    let abs =  Lib.Sequence.index (as_seq h1 out) (2 * v i) in 
+    (if v sign = 0 then (w0 % (2 * m) - m) == v abs else - (w0 % (2 * m) - m) == v abs) /\
+    wUpd < 2 * m /\ 
+    wUpd == scalar_as_nat (as_seq h0 scalar) % pow2 (k * w + w + 1) / pow2 (k * w) / 2 * 2 + 1))
+
+
+let scalar_rwnaf_step #c out scalar window mask r i = 
+    let h0 = ST.get() in 
+  let wVar = to_u64 (index window (size 0)) in 
+    assert(v wVar = v (Lib.Sequence.index (as_seq h0 window) 0));
+
+  let wMask = logand wVar mask in 
+    logand_mask wVar mask (v radix + 1); 
+    FStar.Math.Lemmas.pow2_double_sum (v radix); 
+  scalar_rwnaf_step_compute_di wMask out mask r i; 
+    let h1 = ST.get() in 
+  let d = wMask -. dradix in 
+  let wStart = shift_right (wVar -. d) radix_shiftval in 
+  
+  FStar.Math.Lemmas.lemma_div_lt_nat (v (wVar -. d)) 64 (v radix_shiftval);
+
+  let w0 = scalar_rwnaf_step_compute_window wStart scalar i in 
+  upd window (size 0) w0;
+
+  let h2 = ST.get() in 
+  
+  let d_i = v wVar % (2 * m) - m in 
+  
+  assert(
+    let w0 = v (Lib.Sequence.index (as_seq h0 window) 0) in
+    let sign = Lib.Sequence.index (as_seq h2 out) (2 * v i + 1) in 
+    let abs =  Lib.Sequence.index (as_seq h2 out) (2 * v i) in 
+    if v sign = 0 then (w0 % (2 * m) - m) == v abs else - (w0 % (2 * m) - m) == v abs);
+
+    
+    assert (v wStart = (v wVar - (d_i % pow2 64)) % pow2 64 / m);
+    lemma_mod_sub_distr (v wVar)  (d_i) (pow2 64); 
+    assert (v wStart = (v wVar - d_i) % pow2 64 / m);
+     
+    assert (v wStart =  (v wVar - v wVar % (2 * m) + m) % pow2 64  / m);
+
+    small_mod ((v wVar / (2 * m) * (2 * m)) + m) (pow2 64);
+
+    assert (v wStart =  v wVar / (2 * m) * 2 + 1);
+
+    pow2_multiplication_modulo_lemma_2 (scalar_as_nat (as_seq h0 scalar) / pow2 ((v i + 1) * w  + 1)) (w + 1) 1;
+
+    assert(scalar_as_nat (as_seq h0 scalar) / pow2 ((v i + 1) * w  + 1) % m * 2 + (v wVar / (2 * m) * 2 + 1) == v w0);
+    assert(scalar_as_nat (as_seq h0 scalar) / pow2 ((v i + 1) * w  + 1) * 2 % pow2 (w + 1)  + (v wVar / (2 * m) * 2 + 1) == v w0);
+    
+    assert(v wVar < 2 * m);
+      small_division_lemma_1 (v wVar) (2 * m);
+    assert(v wVar / (2 * m) == 0);
+
+
+  
+ (** **)   assert(2 * (scalar_as_nat (as_seq h0 scalar) / pow2 ((v i + 1) * w  + 1)) % (2 * m) + 1 == v w0);
+
+    pow2_plus (v i * w) (w + 1); 
+    division_multiplication_lemma (scalar_as_nat (as_seq h0 scalar)) (pow2 (w + 1)) (pow2 (v i * w));
+
+
+
+    division_multiplication_lemma (scalar_as_nat (as_seq h0 scalar)  / (pow2 w)) 2 (pow2 (v i * w));
+    pow2_double_mult (v i * w);
+    assert((scalar_as_nat (as_seq h0 scalar)  / (pow2 w) / (2 * pow2 (v i * w))) % (pow2 w) * 2 + 1 == v w0);
+    
+    assert ((scalar_as_nat (as_seq h0 scalar)  / (pow2 w) / (pow2 (v i * w + 1))) % (pow2 w) * 2 + 1 == v w0);
+
+
+    pow2_modulo_division_lemma_1 (scalar_as_nat (as_seq h0 scalar)  / pow2 w) (v i * w + 1) (v i * w + 1 + w);
+
+    pow2_double_mult (v i * w); 
+    
+    division_multiplication_lemma (scalar_as_nat (as_seq h0 scalar)  / (pow2 w)  % pow2 (v i * w + 1 + w)) (pow2 (v i * w)) (pow2 1);
+
+   assert(scalar_as_nat (as_seq h0 scalar)  / (pow2 w)  % pow2 (v i * w + 1 + w) / pow2 (v i * w) / pow2 1  * 2 + 1 == v w0);
+
+   let k = v i + 1 in 
+   
+   assert(2 * (scalar_as_nat (as_seq h0 scalar) / pow2 (k * w  + 1)) % (pow2 (w + 1)) + 1 == v w0);
+   
+
+   assert(scalar_as_nat (as_seq h0 scalar) / pow2 (k * w  + 1) % pow2 w * 2 + 1 == v w0);
+
+   pow2_modulo_division_lemma_1 (scalar_as_nat (as_seq h0 scalar)) (k * w + 1) (k * w + 1 + w);
+   pow2_double_mult (k * w);
+   division_multiplication_lemma (scalar_as_nat (as_seq h0 scalar) % pow2 (k * w + w + 1)) (pow2 (k * w)) 2;
+   
+   assert(scalar_as_nat (as_seq h0 scalar) % pow2 (k * w + w + 1) / pow2 (k * w) / 2 * 2 + 1 == v w0);
+   assert(v w0 < 2 * m)
+    
+
+
+val scalar_rwnaf_lemma0: #c: curve -> scalar: scalar_bytes #c 
+  -> Lemma (scalar_as_nat scalar % pow2 8 = v (Lib.Sequence.index scalar (v (getScalarLenBytes c) - 1)))
+
+let scalar_rwnaf_lemma0 #c scalar = 
+  let len = v (getScalarLen c) in 
+
+  let i0 = ith_bit scalar 0 in 
+  let i1 = ith_bit scalar 1 in 
+  let i2 = ith_bit scalar 2 in 
+  let i3 = ith_bit scalar 3 in 
+  let i4 = ith_bit scalar 4 in  
+  let i5 = ith_bit scalar 5 in 
+  let i6 = ith_bit scalar 6 in  
+  let i7 = ith_bit scalar 7 in  
+
+  let q = v (getScalarLenBytes c) - 1 in
+
+
+  shift_right_lemma (Lib.Sequence.index scalar (v (getScalarLenBytes c) - 1)) (size 0);
+  logand_mask (Lib.Sequence.index scalar  (v (getScalarLenBytes c) - 1)) (u8 1) 1; 
+
+  assert(v i0 == v (Lib.Sequence.index scalar q) % 2);
+  assume (v i0 + v i1 * pow2 1 + v i2 * pow2 2 + v i3 * pow2 3 + v i4 * pow2 4 + v i5 * pow2 5 + v i6 * pow2 6 + v i7  * pow2 7== v (Lib.Sequence.index scalar q));
+
+  assert_norm (pow2 2 = 4);
+  assert_norm (pow2 3 = 8);
+  assert_norm (pow2 4 = 16);
+  assert_norm (pow2 5 = 32);
+  assert_norm (pow2 6 = 64);
+  assert_norm (pow2 7 = 128);
+  assert_norm (pow2 8 = 256);
+
+
+  scalar_as_nat_def #c scalar len;
+  scalar_as_nat_def #c scalar (len - 1);
+  scalar_as_nat_def #c scalar (len - 2);
+  scalar_as_nat_def #c scalar (len - 3);
+  scalar_as_nat_def #c scalar (len - 4);
+  scalar_as_nat_def #c scalar (len - 5);
+  scalar_as_nat_def #c scalar (len - 6);
+  scalar_as_nat_def #c scalar (len - 7);
+
+  lemma_mod_plus (v (Lib.Sequence.index scalar q)) (scalar_as_nat_ scalar (len - 8)) (pow2 8);
+  assert ( v (Lib.Sequence.index scalar q) < pow2 8);
+  small_mod (v (Lib.Sequence.index scalar q)) (pow2 8);
+
+  assert(scalar_as_nat scalar % pow2 8 = v (Lib.Sequence.index scalar q))
+
+
+
+val logor_mask: a: uint64 -> Lemma (v (logor (u64 1) a) == v a / 2 * 2 + 1)
+
+let logor_mask a = 
+  if v a % 2 = 0 then 
+    begin
+      logor_disjoint (u64 1) a 1;
+      assert(v a + 1 == v (logor (u64 1) a))
+    end
+  else
+    begin
+      assume (v (logor (u64 1) a) == v a)
+    end
+
+
+val scalar_rwnaf_loop: out: lbuffer uint64 (size 104) -> scalar: lbuffer uint8 (size 32) 
+  -> mask: uint64 {v mask = pow2 (v radix + 1) - 1}
+  -> window: lbuffer uint64 (size 1) -> 
+  Stack unit 
+  (requires fun h -> live h out /\ live h scalar /\ live h window /\ 
+    LowStar.Monotonic.Buffer.all_disjoint [loc out; loc scalar; loc window] /\ (
+    let w0 = v (Lib.Sequence.index (as_seq h window) 0) in 
+    w0 == scalar_as_nat #P256 (as_seq h scalar) % pow2 (w + 1) / 2 * 2 + 1 /\
+    w0 < 2 * m))
+  (ensures fun h0 _ h1 -> modifies (loc out |+| loc window) h0 h1 /\ (
+    forall (j: nat {j < 50}). 
+      v (Lib.Sequence.index (as_seq h1 out) j) == (2 * (scalar_as_nat #P256 (as_seq h0 scalar) / 2) / pow2 (w * j) + 1) % (2 * m) - m) /\ (
+    let w0 = v (Lib.Sequence.index (as_seq h1 window) 0) in 
+    w0 == scalar_as_nat #P256 (as_seq h0 scalar) % pow2 (50 * w + w + 1) / pow2 (50 * w) / 2 * 2 + 1 /\
+    w0 < 2 * m))
+
+
+(* to check that the second is the out *)
+let scalar_rwnaf_loop out scalar mask window = 
+  push_frame(); 
+  let r = create (size 1) (u64 0) in 
+    let h0 = ST.get() in 
+  
+  let inv h (i:nat {i <= 50}) = 
+    live h out /\ live h scalar /\ live h window /\ live h r /\
+    modifies (loc out |+| loc window |+| loc r) h0 h /\ (
+    let w0 = v (Lib.Sequence.index (as_seq h window) 0) in 
+    w0 == scalar_as_nat #P256 (as_seq h0 scalar) % pow2 (i * w + w + 1) / pow2 (i * w) / 2 * 2 + 1 /\
+    w0 < 2 * m /\ (
+    forall (j: nat {j < i}). 
+      v (Lib.Sequence.index (as_seq h out) j) == (2 * (scalar_as_nat #P256 (as_seq h0 scalar) / 2) / pow2 (w * j) + 1) % (2 * m) - m)) in  
+
+  Lib.Loops.for 0ul 50ul inv (fun i -> 
+    admit();
+    let h0_ = ST.get() in 
+    scalar_rwnaf_step #P256 out scalar window mask r i;
+    let h1_ = ST.get() in 
+    
+    assert(
+      let w0 = scalar_as_nat #P256 (as_seq h0 scalar) % pow2 (v i * w + w + 1) / pow2 (v i * w) / 2 * 2 + 1 in
+      let wUpd = v (Lib.Sequence.index (as_seq h1_ window) 0) in
+      let sign = Lib.Sequence.index (as_seq h1_ out) (2 * v i + 1) in 
+      let abs =  Lib.Sequence.index (as_seq h1_ out) (2 * v i) in 
+      if v sign = 0 then (w0 % (2 * m) - m) == v abs else - (w0 % (2 * m) - m) == v abs /\
+      wUpd < 2 * m /\ 
+      wUpd == scalar_as_nat #P256 (as_seq h0 scalar) % pow2 ((v i + 1) * w + w + 1) / pow2 ((v i + 1)  * w) / 2 * 2 + 1)
+
+  );
+
+  let h1 = ST.get() in 
+  assert(inv h1 50);
+  assert(forall (j: nat {j < 50}). 
+      v (Lib.Sequence.index (as_seq h1 out) j) == (2 * (scalar_as_nat #P256 (as_seq h0 scalar) / 2) / pow2 (w * j) + 1) % (2 * m) - m);
+  pop_frame()
+
 
 
 val scalar_rwnaf : out: lbuffer uint64 (size 104) -> scalar: lbuffer uint8 (size 32) -> 
@@ -115,24 +447,37 @@ val scalar_rwnaf : out: lbuffer uint64 (size 104) -> scalar: lbuffer uint8 (size
 let scalar_rwnaf out scalar = 
   push_frame();
 
+  let h0 = ST.get() in 
   let in0 = to_u64 (index scalar (size 31)) in 
   let mask = dradix_wnaf -! (u64 1) in 
   let windowStartValue = logor (u64 1) (logand in0 mask) in 
+
+  assert_norm (pow2 6 == 64);
+    logand_mask in0 mask 6;
+    scalar_rwnaf_lemma0 #P256 (as_seq h0 scalar); 
+    logor_mask (logand in0 mask); 
+    pow2_modulo_modulo_lemma_1 (scalar_as_nat #P256 (as_seq h0 scalar)) 6 8;
+
+
+  assert(v windowStartValue == scalar_as_nat #P256 (as_seq h0 scalar) % pow2 6 / 2 * 2 + 1);
+  multiply_fractions (scalar_as_nat #P256 (as_seq h0 scalar) % pow2 6) 2;
+  pow2_double_mult w;
   
+
   let window = create (size 1) windowStartValue in 
 
   let r = create (size 1) (u64 0) in 
-  let r1 = create (size 1) (u64 0) in 
 
   let h0 = ST.get() in 
-  let inv h1 (i:nat) = live h1 window /\ live h1 out in  
+
+  scalar_rwnaf_loop out scalar mask window; 
+
 
 
   admit();
 
-  Lib.Loops.for 0ul 50ul inv
-    (fun i -> scalar_rwnaf_step out scalar window mask r i
-  );
+
+
 
   let i = size 50 in 
   
@@ -148,10 +493,6 @@ let scalar_rwnaf out scalar =
 
   upd out (size 2 *! i) r3;
   upd out (size 2 *! i +! size 1) cAsFlag;
-
-
-
-
 
   let d = w -! dradix in 
 
